PropertiesCTR.v
@@ -4,28 +4,144 @@ From Elo Require Import Map.
 From Elo Require Import Core.
 From Elo Require Import CoreExt.
 
+From Elo Require Import Meta.
+
 From Elo Require Import Definitions.
+
+(* ------------------------------------------------------------------------- *)
+(* misc. properties                                                          *)
+(* ------------------------------------------------------------------------- *)
+
+Inductive consistently_typed_effect (m : mem) : effect -> Prop :=
+  | cte_none :
+    consistently_typed_effect m EF_None
+
+  | cte_alloc : forall ad v T,
+    consistently_typed_effect m (EF_Alloc ad v T)
+
+  | cte_read : forall ad v,
+    consistently_typed_effect m (EF_Read ad v)
+
+  | cte_write : forall ad v T,
+    ad < #m ->
+    empty |-- v is T ->
+    empty |-- m[ad].tm is T ->
+    m[ad].typ = <{{&T}}> ->
+    consistently_typed_effect m (EF_Write ad v <{{&T}}>)
+
+  | cte_spawn : forall t,
+    consistently_typed_effect m (EF_Spawn t)
+  .
+
+Lemma cte_tstep_write_T : forall m t t' ad v T Tv,
+  well_typed_term t ->
+  consistently_typed_references m t ->
+  (* --- *)
+  empty |-- v is Tv ->
+  t --[EF_Write ad v T]--> t' ->
+  T = <{{&Tv}}>.
+Proof.
+  intros * [T' ?] **. generalize dependent T'.
+  induction_tstep; intros; inv_type; inv_ctr; eauto.
+  inv_type. inv_ctr. apply_deterministic_typing. eauto.
+Qed.
+
+Lemma cte_tstep_preservation : forall m t t' e,
+  valid_addresses m t ->
+  well_typed_term t ->
+  consistently_typed_references m t ->
+  (* --- *)
+  t --[e]--> t' ->
+  exists m', consistently_typed_effect m' e.
+Proof.
+  intros. destruct e;
+  try solve [exists m; eauto using consistently_typed_effect].
+  assert (ad < #m) by eauto using vad_tstep_write_address_length.
+  assert (well_typed_term v) as [Tv ?] by eauto using wtt_tstep_write_value.
+  assert (T = <{{&Tv}}>) by eauto using cte_tstep_write_T. subst.
+  exists (m[ad <- (v, <{{&Tv}}>)]).
+  eapply cte_write; eauto; try solve [simpl_array; trivial].
+  rewrite set_preserves_length. assumption.
+Qed.
+
+Lemma cte_tstep_write : forall m t t' ad v T,
+  valid_addresses m t ->
+  well_typed_term t ->
+  consistently_typed_references m t ->
+  (* --- *)
+  t --[EF_Write ad v T]--> t' ->
+  consistently_typed_effect m[ad <- (v, T)] (EF_Write ad v T).
+Proof.
+  intros.
+  assert (ad < #m) by eauto using vad_tstep_write_address_length.
+  assert (well_typed_term v) as [Tv ?] by eauto using wtt_tstep_write_value.
+  assert (T = <{{&Tv}}>) by eauto using cte_tstep_write_T. subst.
+  eapply cte_write; eauto; try solve [simpl_array; trivial].
+  rewrite set_preserves_length. assumption.
+Qed.
+
+(* ------------------------------------------------------------------------- *)
+(* TODO                                                                      *)
+(* ------------------------------------------------------------------------- *)
+
+(*
+Lemma ctr_tstep_write_consistent_memval : forall m t t' ad v T Tv,
+  well_typed_term t ->
+  consistently_typed_references m t ->
+  (* --- *)
+  empty |-- v is Tv ->
+  t --[EF_Write ad v T]--> t' ->
+  empty |-- m[ad].tm is Tv.
+Proof.
+  intros * [T' ?] **. generalize dependent T'.
+  induction_tstep; intros; inv_type; inv_ctr; eauto.
+  inv_type. inv_ctr. apply_deterministic_typing. assumption.
+Qed.
+
+Lemma ctr_tstep_write_consistent_memtyp_v : forall m t t' ad v T Tv,
+  well_typed_term t ->
+  consistently_typed_references m t ->
+  (* --- *)
+  empty |-- v is Tv ->
+  t --[EF_Write ad v T]--> t' ->
+  m[ad].typ = <{{&Tv}}>.
+Proof.
+  intros * [T' ?] **. generalize dependent T'.
+  induction_tstep; intros; inv_type; inv_ctr; eauto.
+  inv_type. inv_ctr. apply_deterministic_typing. assumption.
+Qed.
+
+Lemma ctr_tstep_write_consistent_memtyp_T : forall m t t' ad v T,
+  well_typed_term t ->
+  consistently_typed_references m t ->
+  (* --- *)
+  t --[EF_Write ad v T]--> t' ->
+  m[ad].typ = T.
+Proof.
+  intros * [T' ?] **. generalize dependent T'.
+  induction_tstep; intros; inv_type; inv_ctr; eauto.
+  inv_type. inv_ctr. assumption.
+Qed.
+
+Corollary ctr_tstep_write_consistently_typed_effect : forall m t t' ad v T Tv,
+  well_typed_term t ->
+  consistently_typed_references m t ->
+  (* --- *)
+  empty |-- v is Tv ->
+  t --[EF_Write ad v T]--> t' ->
+  T = <{{&Tv}}>.
+Proof.
+  intros. symmetry.
+  erewrite <- ctr_tstep_write_consistent_memtyp_T; eauto.
+  erewrite ctr_tstep_write_consistent_memtyp_v; eauto.
+Qed.
+*)
 
 (* ------------------------------------------------------------------------- *)
 (* preservation                                                              *)
 (* ------------------------------------------------------------------------- *)
 
 Module Preservation.
-
-  (* auxiliary. *)
-  Local Lemma step_write_wtt : forall m t t' ad v Tr T,
-    empty |-- t is T ->
-    t --[EF_Write ad v Tr]--> t' ->
-    consistently_typed_references m t ->
-    (Tr = m[ad].typ /\ exists V, empty |-- v is V /\ empty |-- m[ad].tm is V).
-  Proof.
-    intros * ? ?.
-    assert (exists V, empty |-- v is V) as [? ?].
-    { generalize dependent T. induction_tstep; intros; inv_type; eauto. }
-    intros. generalize dependent T.
-    induction_tstep; intros; inv_type; inv_ctr; eauto.
-    inv_type. inv_ctr. apply_deterministic_typing. eauto.
-  Qed.
 
   (* subst & mem ----------------------------------------------------------- *)
 
@@ -47,7 +163,7 @@ Module Preservation.
   Proof.
     intros. induction t; eauto using consistently_typed_references;
     inv_vad; inv_ctr; eauto using consistently_typed_references;
-    (eapply ctr_refM || eapply ctr_refI); simpl_array; assumption.
+    (eapply ctr_adM || eapply ctr_adI); simpl_array; assumption.
   Qed.
 
   Lemma ctr_mem_set_preservation : forall m t ad v T,
@@ -58,13 +174,28 @@ Module Preservation.
     consistently_typed_references m t ->
     consistently_typed_references m[ad <- (v, m[ad].typ)] t.
   Proof.
-    intros. induction t;
-    eauto using consistently_typed_references;
+    intros. induction t; eauto using consistently_typed_references;
     inv_ctr; eauto using consistently_typed_references;
     match goal with _ : _[?ad].typ = _ |- _ => rename ad into ad' end;
-    (eapply ctr_refM || eapply ctr_refI);
-    decompose sum (lt_eq_lt_dec ad' ad); subst;
-    simpl_array; trivial; apply_deterministic_typing; trivial.
+    (eapply ctr_adM || eapply ctr_adI);
+    decompose sum (lt_eq_lt_dec ad' ad); subst; simpl_array;
+    trivial; apply_deterministic_typing; trivial.
+  Qed.
+
+  Lemma ctr_mem_set_preservation2 : forall m t ad v T Tv,
+    ad < #m ->
+    empty |-- v is Tv ->
+    empty |-- m[ad].tm is Tv ->
+    T = m[ad].typ ->
+    (* --- *)
+    consistently_typed_references m t ->
+    consistently_typed_references m[ad <- (v, T)] t.
+  Proof.
+    intros. induction t; eauto using consistently_typed_references;
+    inv_ctr; eauto using consistently_typed_references;
+    (eapply ctr_adM || eapply ctr_adI);
+    destruct (nat_eq_dec ad n); subst; simpl_array; trivial;
+    apply_deterministic_typing; trivial.
   Qed.
 
   (* tstep ----------------------------------------------------------------- *)
@@ -78,7 +209,7 @@ Module Preservation.
     inv_ctr. eauto using ctr_subst_preservation.
   Qed.
 
-  Local Lemma ctr_tstep_alloc_preservation : forall m t t' v T,
+  Lemma ctr_tstep_alloc_preservation : forall m t t' v T,
     valid_addresses m t ->
     well_typed_term t ->
     (* --- *)
@@ -89,11 +220,12 @@ Module Preservation.
     intros * ? [T' ?] **. generalize dependent T'.
     induction_tstep; intros; inv_vad; inv_type; inv_ctr;
     eauto using consistently_typed_references, ctr_mem_add_preservation;
-    (eapply ctr_refM || eapply ctr_refI); simpl_array; trivial.
+    (eapply ctr_adM || eapply ctr_adI); simpl_array; trivial.
   Qed.
 
-  Local Lemma ctr_tstep_read_preservation : forall m t t' ad v,
+  Lemma ctr_tstep_read_preservation : forall m t t' ad v,
     consistently_typed_references m v ->
+    (* --- *)
     consistently_typed_references m t ->
     t --[EF_Read ad v]--> t' ->
     consistently_typed_references m t'.
@@ -102,22 +234,41 @@ Module Preservation.
     eauto using consistently_typed_references.
   Qed.
 
-  Local Lemma ctr_tstep_write_preservation : forall m t t' ad v T,
-    well_typed_term t ->
+  Lemma ctr_tstep_write_preservation : forall m t t' ad v T,
     valid_addresses m t ->
+    well_typed_term t ->
+    (* --- *)
     consistently_typed_references m t ->
     t --[EF_Write ad v T]--> t' ->
     consistently_typed_references m[ad <- (v, T)] t'.
   Proof.
-    intros * [T' ?]. intros. assert (
-      T = m[ad].typ /\
-      exists Tv, empty |-- v is Tv /\ empty |-- m[ad].tm is Tv)
-      as [? [? [? ?]]] by eauto using step_write_wtt.
+    intros * ? Hwtt **. inversion Hwtt as [T' ?]. generalize dependent T'.
+    induction_tstep; intros; inv_vad; inv_wtt; inv_ctr;
+    eauto using consistently_typed_references.
+    - eapply 
+
+      assert (exists m', consistently_typed_effect m' (EF_Write ad v T))
+        as [? ?] by eauto using cte_tstep_preservation.
+
+
+
+
+
+    (*
+    assert (
+      T = m[ad].typ /\ exists Tv, empty |-- v is Tv /\ empty |-- m[ad].tm is Tv)
+      as [? [? [? ?]]] by admit.
+    *)
     generalize dependent T'.
-    induction_tstep; intros; inv_type; inv_vad; inv_ctr;
-    eauto using valid_address_write,
-      consistently_typed_references,
-      ctr_mem_set_preservation.
+    induction_tstep; intros; inv_vad; inv_type; inv_ctr;
+    eauto using ctr_mem_set_preservation,
+      vad_tstep_write_address_length,
+      consistently_typed_references.
+    - eapply ctr_asg.
+      + eapply IHtstep; eauto.
+      + eapply ctr_mem_set_preservation2; eauto;
+        eauto using vad_tstep_write_address_length.
+        eauto uding
   Qed.
 
   Lemma ctr_tstep_spawn_preservation : forall m t t' block,
@@ -129,24 +280,27 @@ Module Preservation.
     eauto using consistently_typed_references.
   Qed.
 
-  Local Corollary ctr_mstep_preservation : forall m m' t t' e,
-    well_typed_term t ->
-    valid_addresses m t ->
+  (* mstep ----------------------------------------------------------------- *)
+
+  Corollary ctr_mstep_preservation : forall m m' t t' e,
     forall_memory m (consistently_typed_references m) ->
+    valid_addresses m t ->
+    well_typed_term t ->
+    (* --- *)
     consistently_typed_references m t ->
     m / t ==[e]==> m' / t' ->
     consistently_typed_references m' t'.
   Proof.
-    solve_mstep_preservation_using
-      ctr_tstep_none_preservation
-      ctr_tstep_alloc_preservation
-      ctr_tstep_read_preservation
-      ctr_tstep_write_preservation.
+    intros. inv_mstep;
+    eauto using ctr_tstep_none_preservation,
+                ctr_tstep_alloc_preservation,
+                ctr_tstep_read_preservation,
+                ctr_tstep_write_preservation.
   Qed.
 
-  (* ------------------------------------------------------------------------- *)
+  (* cstep ----------------------------------------------------------------- *)
 
-  Local Lemma ctr_thread_default_preservation : forall m,
+  Lemma ctr_thread_default : forall m,
     consistently_typed_references m thread_default.
   Proof.
     eauto using consistently_typed_references.
@@ -160,16 +314,17 @@ Module Preservation.
     intros. induction_tstep; inv_ctr; eauto.
   Qed.
 
-  Local Lemma ctr_untouched_threads_preservation : forall m m' ths tid tid' e t',
-    forall_threads ths well_typed_term ->
+  Lemma ctr_untouched_threads_preservation : forall m m' ths tid tid' t' e,
     forall_threads ths (valid_addresses m) ->
+    forall_threads ths well_typed_term ->
     forall_threads ths (consistently_typed_references m) ->
+    (* --- *)
     tid <> tid' ->
     tid' < #ths ->
     m / ths[tid] ==[e]==> m' / t' ->
     consistently_typed_references m' ths[tid'].
   Proof.
-    intros *. intros Htype. intros. destruct (Htype tid).
+    intros * ? Htype **. destruct (Htype tid).
     inv_mstep; eauto using ctr_mem_add_preservation.
     match goal with
     | _ : _ --[EF_Write _ _ ?T]--> _ |- _ =>
@@ -182,127 +337,110 @@ Module Preservation.
   Qed.
 
   Corollary ctr_cstep_preservation : forall m m' ths ths' tid e,
-    forall_threads ths well_typed_term ->
     forall_threads ths (valid_addresses m) ->
+    forall_threads ths well_typed_term ->
+    (* --- *)
     forall_memory m (consistently_typed_references m) ->
     forall_threads ths (consistently_typed_references m) ->
     m / ths ~~[tid, e]~~> m' / ths' ->
     forall_threads ths' (consistently_typed_references m').
   Proof.
-    intros * Htype ?. destruct (Htype tid).
-    eauto 6 using cstep_preservation,
-      ctr_tstep_spawn_preservation,
-      ctr_mstep_preservation,
-      ctr_thread_default_preservation,
-      ctr_spawn_block,
-      ctr_untouched_threads_preservation.
+    intros * ? Htype **. destruct (Htype tid).
+    eapply cstep_preservation;
+    eauto using ctr_tstep_spawn_preservation,
+                ctr_mstep_preservation,
+                ctr_thread_default,
+                ctr_spawn_block,
+                ctr_untouched_threads_preservation.
   Qed.
 
-(* ------------------------------------------------------------------------- *)
+  (* tstep mem ------------------------------------------------------------- *)
 
-Local Lemma wtt_alloc_value_generalization : forall t t' ad v T,
-  well_typed_term t ->
-  t --[EF_Alloc ad v T]--> t' ->
-  well_typed_term v.
-Proof.
-  unfold well_typed_term. intros * [T' ?]. intros. generalize dependent T'.
-  induction_tstep; intros; inv_type; eauto.
-Qed.
+  Lemma ctr_tstep_alloc_mem_preservation : forall m t t' v T,
+    forall_memory m (valid_addresses m) ->
+    valid_addresses m t ->
+    well_typed_term t ->
+    (* --- *)
+    forall_memory m (consistently_typed_references m) ->
+    consistently_typed_references m t ->
+    t --[EF_Alloc (#m) v T]--> t' ->
+    forall_memory (m +++ (v, T)) (consistently_typed_references (m +++ (v, T))).
+  Proof.
+    intros ** ad.
+    assert (well_typed_term v) as [? ?] by eauto using wtt_tstep_alloc_value.
+    decompose sum (lt_eq_lt_dec ad (#m)); subst; simpl_array;
+    eauto using consistently_typed_references; (* optimization *)
+    eauto using ctr_mem_add_preservation, ctr_tstep_alloc_value.
+  Qed.
 
-Local Lemma ctr_alloc_value_generalization : forall m t t' ad v T,
-  consistently_typed_references m t ->
-  t --[EF_Alloc ad v T]--> t' ->
-  consistently_typed_references m v.
-Proof.
-  intros. induction_tstep; intros; inv_ctr; eauto.
-Qed.
+  Lemma ctr_tstep_write_mem_preservation : forall m t t' ad v T,
+   valid_addresses m t ->
+   well_typed_term t ->
+   (* --- *)
+   forall_memory m (consistently_typed_references m) ->
+   consistently_typed_references m t ->
+   t --[EF_Write ad v T]--> t' ->
+   forall_memory m[ad <- (v, T)] (consistently_typed_references m[ad <- (v, T)])
+   .
+  Proof.
+    intros * ? [? ?] **. intros ad'.
+    assert (ad < #m) by eauto using vad_tstep_write_address_length.
+    match goal with
+    | _ : _ --[EF_Write _ _ ?T]--> _ |- _ =>
+      assert (
+        T = m[ad].typ /\
+        exists V, empty |-- v is V /\ empty |-- m[ad].tm is V)
+        as [? [? [? ?]]] by eauto using step_write_wtt
+    end.
+    decompose sum (lt_eq_lt_dec ad' ad); subst; simpl_array;
+    eauto using ctr_mem_set_preservation, ctr_tstep_write_value.
+  Qed.
 
-Local Lemma ctr_write_value_generalization : forall m t t' ad v T,
-  consistently_typed_references m t ->
-  t --[EF_Write ad v T]--> t' ->
-  consistently_typed_references m v.
-Proof.
-  intros. induction_tstep; intros; inv_ctr; eauto.
-Qed.
+  (* mstep mem ------------------------------------------------------------- *)
 
-Local Lemma ctr_tstep_alloc_mem_preservation : forall m t t' v T,
-  well_typed_term t ->
-  valid_addresses m t ->
-  forall_memory m (valid_addresses m) ->
-  (* --- *)
-  consistently_typed_references m t ->
-  forall_memory m (consistently_typed_references m) ->
-  t --[EF_Alloc (#m) v T]--> t' ->
-  forall_memory (m +++ (v, T)) (consistently_typed_references (m +++ (v, T))).
-Proof.
-  intros. intros ad.
-  assert (well_typed_term v) as [? ?]
-    by eauto using wtt_alloc_value_generalization.
-  decompose sum (lt_eq_lt_dec ad (#m)); subst; simpl_array;
-  eauto using consistently_typed_references; (* optimization *)
-  eauto using ctr_mem_add_preservation, ctr_alloc_value_generalization.
-Qed.
+  Corollary ctr_mstep_mem_preservation : forall m m' t t' e,
+    well_typed_term t ->
+    valid_addresses m t ->
+    forall_memory m (valid_addresses m) ->
+    (* --- *)
+    forall_memory m (consistently_typed_references m) ->
+    consistently_typed_references m t ->
+    m / t ==[e]==> m' / t' ->
+    forall_memory m' (consistently_typed_references m').
+  Proof.
+    intros. inv_mstep; eauto using ctr_tstep_alloc_mem_preservation,
+                                   ctr_tstep_write_mem_preservation.
+  Qed.
 
-Local Lemma ctr_tstep_write_mem_preservation : forall m t t' ad v T,
-  ad < # m ->
-  well_typed_term t ->
-  (* --- *)
-  consistently_typed_references m t ->
-  forall_memory m (consistently_typed_references m) ->
-  t --[EF_Write ad v T]--> t' ->
-  forall_memory m[ad <- (v, T)] (consistently_typed_references m[ad <- (v, T)]).
-Proof.
-  intros * ? [? ?]. intros. intros ad'.
-  match goal with
-  | _ : _ --[EF_Write _ _ ?T]--> _ |- _ =>
-    assert (
-      T = m[ad].typ /\
-      exists V, empty |-- v is V /\ empty |-- m[ad].tm is V)
-      as [? [? [? ?]]] by eauto using step_write_wtt
-  end.
-  decompose sum (lt_eq_lt_dec ad' ad); subst; simpl_array;
-  eauto using ctr_write_value_generalization, ctr_mem_set_preservation.
-Qed.
+  (* cstep mem ------------------------------------------------------------- *)
 
-Local Corollary ctr_mstep_mem_preservation : forall m m' t t' e,
-  well_typed_term t ->
-  valid_addresses m t ->
-  forall_memory m (valid_addresses m) ->
-  (* --- *)
-  consistently_typed_references m t ->
-  forall_memory m (consistently_typed_references m) ->
-  m / t ==[e]==> m' / t' ->
-  forall_memory m' (consistently_typed_references m').
-Proof.
-  solve_mstep_mem_preservation_using 
-    ctr_tstep_alloc_mem_preservation 
-    ctr_tstep_write_mem_preservation.
-Qed.
+  Corollary ctr_cstep_mem_preservation : forall m m' ths ths' tid e,
+    forall_memory m (valid_addresses m) ->
+    forall_threads ths (valid_addresses m) ->
+    forall_threads ths well_typed_term ->
+    (* --- *)
+    forall_memory m (consistently_typed_references m) ->
+    forall_threads ths (consistently_typed_references m) ->
+    m / ths ~~[tid, e]~~> m' / ths' ->
+    forall_memory m' (consistently_typed_references m').
+  Proof.
+    intros. inv_cstep; eauto using ctr_mstep_mem_preservation.
+  Qed.
 
-Local Corollary ctr_cstep_mem_preservation : forall m m' ths ths' tid e,
-  forall_threads ths well_typed_term ->
-  forall_threads ths (valid_addresses m) ->
-  forall_memory m (valid_addresses m) ->
-  (* --- *)
-  forall_threads ths (consistently_typed_references m) ->
-  forall_memory m (consistently_typed_references m) ->
-  m / ths ~~[tid, e]~~> m' / ths' ->
-  forall_memory m' (consistently_typed_references m').
-Proof.
-  solve_cstep_mem_preservation_using ctr_mstep_mem_preservation.
-Qed.
+  (* consistently-typed-references preservation ---------------------------- *)
 
-(* ------------------------------------------------------------------------- *)
+  Theorem consistently_typed_references_preservation :
+    forall m m' ths ths' tid e,
+      forall_program m ths (valid_addresses m) ->
+      forall_program m ths well_typed_term ->
+      (* --- *)
+      forall_program m ths (consistently_typed_references m) ->
+      m / ths ~~[tid, e]~~> m' / ths' ->
+      forall_program m' ths' (consistently_typed_references m').
+  Proof.
+    intros * [? ?] [_ ?] [? ?]. intros.
+    eauto using ctr_cstep_preservation, ctr_cstep_mem_preservation.
+  Qed.
 
-Theorem consistently_typed_references_preservation : forall m m' ths ths' tid e,
-  forall_program m ths well_typed_term ->
-  forall_program m ths (valid_addresses m) ->
-  (* --- *)
-  forall_program m ths (consistently_typed_references m) ->
-  m / ths ~~[tid, e]~~> m' / ths' ->
-  forall_program m' ths' (consistently_typed_references m').
-Proof.
-  intros * [_ ?] [? ?] [? ?]. intros.
-  eauto using ctr_cstep_preservation, ctr_cstep_mem_preservation.
-Qed.
+End Preservation.
 
