CTR.v
@@ -2,6 +2,7 @@ From Elo Require Import Util.
 From Elo Require Import Array.
 From Elo Require Import Map.
 From Elo Require Import Core.
+From Elo Require Import CoreExt.
 
 (* ------------------------------------------------------------------------- *)
 (* consistently-typed-references                                             *)
@@ -14,12 +15,12 @@ Inductive consistently_typed_references (m : mem) : tm -> Prop :=
   | ctr_num : forall n,
     consistently_typed_references m <{N n}>
 
-  | ctr_refM : forall T ad,
+  | ctr_adM : forall T ad,
     empty |-- m[ad].tm is T ->
     m[ad].typ = <{{ &T }}> ->
     consistently_typed_references m <{&ad :: &T}>
 
-  | ctr_refI : forall T ad,
+  | ctr_adI : forall T ad,
     empty |-- m[ad].tm is <{{ Immut T }}> ->
     m[ad].typ = <{{ i&T }}> ->
     consistently_typed_references m <{&ad :: i&T}>
@@ -81,4 +82,24 @@ Local Ltac match_ctr tactic :=
 Ltac inv_ctr := match_ctr inv.
 
 Ltac invc_ctr := match_ctr invc.
+
+(* ------------------------------------------------------------------------- *)
+(* independent properties                                                    *)
+(* ------------------------------------------------------------------------- *)
+
+Lemma ctr_tstep_alloc_value : forall m t t' ad v T,
+  consistently_typed_references m t ->
+  t --[EF_Alloc ad v T]--> t' ->
+  consistently_typed_references m v.
+Proof.
+  intros. induction_tstep; intros; inv_ctr; eauto.
+Qed.
+
+Lemma ctr_tstep_write_value : forall m t t' ad v T,
+  consistently_typed_references m t ->
+  t --[EF_Write ad v T]--> t' ->
+  consistently_typed_references m v.
+Proof.
+  intros. induction_tstep; intros; inv_ctr; eauto.
+Qed.
 
